CleanQ/CleanQ_SimpleQ.thy
@@ -24,12 +24,171 @@
 
 theory CleanQ_SimpleQ
   imports 
-    "../autocorres/autocorres/AutoCorres"
+    "AutoCorres.AutoCorres"
     CleanQ_RB
 begin
 
-external_file "CleanQ_SimpleQ.c"
+(* ==================================================================================== *)
+subsection \<open>Constants and Type Definitions\<close>
+(* ==================================================================================== *)
 
+text \<open>
+  We define a few type synonyms and constants to reason about addresses
+\<close>
+type_synonym ulong_t = "64 word"
+type_synonym uint_t = "32 word"
+type_synonym ushort_t = "16 word"
+
+abbreviation "addrlimit \<equiv> (0xffffffffffffffff::ulong_t)"
+abbreviation "addrlimitnat \<equiv> (0xffffffffffffffff::nat)"
+
+lemma "addrlimit = of_nat addrlimitnat"
+  by(auto)
+lemma "unat (addrlimit) = addrlimitnat"
+  by(auto)
+
+
+declare[[show_types ]]
+sledgehammer_params[timeout = 120, provers = cvc4 z3 spass e remote_vampire vampire]
+  
+
+(* ==================================================================================== *)
+subsection \<open>Helper Lemmas\<close>
+(* ==================================================================================== *)
+
+lemma unat_64word_eq_lt_lt:
+ "unat (C::ulong_t) = ULONG_MAX \<Longrightarrow> (D::ulong_t) < C \<Longrightarrow> unat (D) < ULONG_MAX"
+  by(simp add: word_less_nat_alt)
+
+lemma unat_32word_eq_lt_lt:
+ "unat (C::uint_t) = UINT_MAX \<Longrightarrow> (D::uint_t) < C \<Longrightarrow> unat (D) < UINT_MAX"
+  by(simp add: word_less_nat_alt)
+
+lemma unat_64word_lt_lt_lt:
+ "unat (C::ulong_t) < ULONG_MAX \<Longrightarrow> (D::ulong_t) < C \<Longrightarrow> unat (D) < ULONG_MAX"
+  by(simp add: word_less_nat_alt)
+
+lemma unat_32word_lt_lt_lt:
+ "unat (C::uint_t) < UINT_MAX \<Longrightarrow> (D::uint_t) < C \<Longrightarrow> unat (D) < UINT_MAX"
+  by(simp add: word_less_nat_alt)
+
+lemma unat_64word_leq_lt_lt: 
+  "unat (C::ulong_t) \<le> ULONG_MAX \<Longrightarrow> (D::ulong_t) < C \<Longrightarrow> unat (D) < ULONG_MAX"
+  using unat_64word_eq_lt_lt unat_64word_lt_lt_lt PackedTypes.order_leE 
+  by blast
+
+lemma unat_32word_leq_lt_lt: 
+  "unat (C::uint_t) \<le> UINT_MAX \<Longrightarrow> (D::uint_t) < C \<Longrightarrow> unat (D) < UINT_MAX"
+  using unat_32word_eq_lt_lt unat_32word_lt_lt_lt PackedTypes.order_leE 
+  by blast
+
+lemma unat_64word_lt_succ_leq:
+  "unat (C::ulong_t) \<le> ULONG_MAX \<Longrightarrow> (D::ulong_t) < C \<Longrightarrow> Suc (unat (D)) \<le> ULONG_MAX"
+  using unat_64word_leq_lt_lt  by (simp add: less_eq_Suc_le) 
+
+lemma unat_32word_lt_succ_leq:
+  "unat (C::uint_t) \<le> ULONG_MAX \<Longrightarrow> (D::uint_t) < C \<Longrightarrow> Suc (unat (D)) \<le> UINT_MAX"
+  using unat_32word_leq_lt_lt  by (simp add: less_eq_Suc_le) 
+
+lemma unat_64word_succ_mod:
+  assumes sz: "1 < unat N"  and hlt: "H < N"
+  shows
+  "unat (((H::ulong_t) + 1) mod (N::ulong_t)) = Suc (unat (H)) mod unat (N)"
+  using sz hlt  
+  by (metis add.commute less_is_non_zero_p1 unatSuc unat_mod)
+
+lemma unat_32word_succ_mod:
+  assumes sz: "1 < unat N"  and hlt: "H < N"
+  shows
+  "unat (((H::uint_t) + 1) mod (N::uint_t)) = Suc (unat (H)) mod unat (N)"
+  using sz hlt  
+  by (metis add.commute less_is_non_zero_p1 unatSuc unat_mod)
+
+lemma unat_word_lt: 
+  "a < b \<Longrightarrow> unat a < unat b"
+  by (simp add: unat_mono)
+
+lemma unat_word_leq: 
+  "a \<le> b \<Longrightarrow> unat a \<le> unat b"
+  by (simp add: word_le_nat_alt)
+
+lemma word64_mult_inequality:
+  assumes notzero: "c \<noteq> 0" 
+    and inrangex: "x * unat(c) <  2 ^ 64"
+    and inrangey: "unat(y) * unat(c) <  2 ^ 64"
+    and neq: "x \<noteq> unat y"
+  shows "((of_nat x)::ulong_t) * (c::ulong_t) \<noteq> (y::ulong_t) * (c::ulong_t)"
+proof -
+  from notzero inrangex have xlim:
+    "x < 2 ^ 64"
+    by (metis linorder_neqE_nat multi_lessD not_less0 unat_gt_0)
+
+  have xc_limit:
+    "unat ((of_nat x)::ulong_t) * unat c < 2 ^ 64"
+    using  xlim unat_of_nat64 word_bits_conv inrangex by(auto)
+
+  have xc_equiv:
+    "unat (((of_nat x)::ulong_t) * c) = x * unat c"
+    using xc_limit unat_mult_lem unat_of_nat64 word_bits_conv inrangex by fastforce
+  
+  have yc_equiv: 
+    "unat (y * c) = unat(y) * unat (c)"
+    using inrangey  unat_mult_lem by fastforce
+
+  show ?thesis
+    using xc_equiv yc_equiv neq notzero unat_eq_zero
+    by force
+qed
+
+lemma word64_mult_inequality2:
+  assumes notzero: "c \<noteq> 0" 
+    and inrangex: " x * unat(c) \<le> unat addrlimit"
+    and inrangey: "unat (y) * unat (c) \<le> unat  addrlimit"
+    and neq: "x \<noteq> unat y"
+  shows "((of_nat x)::ulong_t) * (c::ulong_t) \<noteq> (y::ulong_t) * (c::ulong_t)"
+proof -
+  from notzero inrangex have xlim0:
+    "x \<le> unat addrlimit"
+    using dual_order.trans unat_eq_zero by fastforce
+
+  from xlim0 have xlim:
+    "x < 2 ^ 64"
+    by (metis (mono_tags, hide_lams) le_unat_uoi  word_bits_conv unat_less_2p_word_bits)
+
+   from xlim have xc_limit:
+    "unat ((of_nat x)::ulong_t) * unat c < 2 ^ 64"
+     by (metis (no_types, hide_lams) le_unat_uoi unat_less_2p_word_bits
+                                     unat_of_nat64 word_bits_conv inrangex)
+
+    have xc_equiv:
+    "unat (((of_nat x)::ulong_t) * c) = x * unat c"
+    using inrangex le_unat_uoi by fastforce
+  have yc_equiv: 
+    "unat (y * c) = unat(y) * unat (c)"
+    using inrangey le_unat_uoi by fastforce
+
+  show ?thesis
+    using xc_equiv yc_equiv neq notzero unat_eq_zero 
+    by force
+qed
+
+lemma word64_multply_const_equaltiy:
+assumes notzero: "c \<noteq> (0::ulong_t)"
+  and hclimit:  "unat (h) * unat (c) < 2 ^ 64"
+  and xclimit:  "x * unat (c) < 2 ^ 64"
+shows "((of_nat x)::ulong_t) * (c::ulong_t) = (h::ulong_t) * (c::ulong_t) \<longleftrightarrow> x = unat (h)"
+  using hclimit notzero word64_mult_inequality xclimit by fastforce
+
+(* ==================================================================================== *)
+subsection \<open>SimpleQ C Implementation\<close>
+(* ==================================================================================== *)
+
+text \<open>
+  Next we load the CleanQ_SimpleQ.c implementation of a shared-memory ring buffer, and
+  show that the C implementation refines the abstract ring buffer implementation.
+\<close>
+
+external_file "CleanQ_SimpleQ.c"
 install_C_file "CleanQ_SimpleQ.c"
 
 autocorres [
@@ -49,7 +208,7 @@ autocorres [
   (* force_heap_abs = FUNC_NAMES, *)
   (* Attempt _heap abstraction_  on the given list of functions *)
 
-(*  heap_abs_syntax, *)
+  (* heap_abs_syntax, *)
   (* Enable experimental heap abstraction syntactic sugar. *)
 
   (* skip_heap_abs *)
@@ -116,305 +275,112 @@ autocorres [
 ] "CleanQ_SimpleQ.c"
 (* skip_word_abs *)
 
-
-
-record buffer =
-  base :: nat
-  length :: nat
+text \<open>
+ We can now enter the defined context by autocorres. 
+\<close>
 
 context CleanQ_SimpleQ begin
 
-(* Ring Buffer C parser output. *)
-thm rb_init_body_def
-thm rb_can_enq_body_def
-thm rb_can_enq_c_fun_def
-thm rb_can_enq_def
+(* ==================================================================================== *)
+subsection \<open>C Definitions\<close>
+(* ==================================================================================== *)
 
+abbreviation "ERR_OK \<equiv> (0)"
+abbreviation "ERR_QUEUE_FULL \<equiv> (-1)"
+abbreviation "ERR_QUEUE_EMPTY  \<equiv> (-2)"
+abbreviation "ERR_NO_BUFFERS \<equiv> (-3)"
 
-thm rb_enq_body_def
-thm rb_can_deq_body_def
+(* ==================================================================================== *)
+subsection \<open>Invariant\<close>
+(* ==================================================================================== *)
 
-thm rb_deq_body_def
-thm rb_can_enq_body_def
-term rb_C
-term buffer_C
-term head_C
+text \<open>
+  We now define the validity invariant for the ring buffer struct. We first define
+  abbrevations for each of the field
+\<close>
 
-term ring_C
-
-
-(* some helper lemmas with the 64-bit words *)
-
-lemma unat_64word_eq_lt_lt:
- "unat (C :: 64 word) = ULONG_MAX \<Longrightarrow> (D :: 64 word) < C \<Longrightarrow> unat (D) < ULONG_MAX"
-  by(simp add: word_less_nat_alt)
-
-lemma unat_64word_lt_lt_lt:
- "unat (C :: 64 word) < ULONG_MAX \<Longrightarrow> (D :: 64 word) < C \<Longrightarrow> unat (D) < ULONG_MAX"
-  by(simp add: word_less_nat_alt)
-
-lemma unat_64word_leq_lt_lt: 
-  "unat (C :: 64 word) \<le> ULONG_MAX \<Longrightarrow> (D :: 64 word) < C \<Longrightarrow> unat (D) < ULONG_MAX"
-  using unat_64word_eq_lt_lt unat_64word_lt_lt_lt PackedTypes.order_leE 
-  by blast
-
-lemma unat_64word_lt_succ_leq:
-  "unat (C :: 64 word) \<le> ULONG_MAX \<Longrightarrow> (D :: 64 word) < C \<Longrightarrow> Suc (unat (D)) \<le> ULONG_MAX"
-  using unat_64word_leq_lt_lt  by (simp add: less_eq_Suc_le) 
-
-
-
+abbreviation "c_rb_valid_is_valid s rb \<equiv> is_valid_rb_C s rb"
+abbreviation "c_rb_valid_size s rb \<equiv> 1 <  (size_C (heap_rb_C s rb))"
+abbreviation "c_rb_valid_head s rb \<equiv> head_C (heap_rb_C s rb) < size_C (heap_rb_C s rb)"
+abbreviation "c_rb_valid_tail s rb \<equiv> tail_C (heap_rb_C s rb) < size_C (heap_rb_C s rb)"
+abbreviation "c_rb_valid_ring s rb \<equiv> (\<forall>i \<le> uint (size_C (heap_rb_C s rb)). 
+                                    is_valid_buffer_C s (ring_C (heap_rb_C s rb) +\<^sub>p i) \<and>
+                                    ptr_val (ring_C (heap_rb_C s rb) +\<^sub>p i) \<le> addrlimit)"
 
 (* this one should be the pre-condition for the operation *)
-definition rb_valid_c :: " lifted_globals \<Rightarrow> rb_C ptr \<Rightarrow> bool"
-  where "rb_valid_c s rb \<longleftrightarrow> is_valid_rb_C s rb 
-                            \<and> unat (size_C (heap_rb_C s rb)) > 1 
-                            \<and> unat (head_C (heap_rb_C s rb)) < unat(size_C (heap_rb_C s rb))
-                            \<and> unat (tail_C (heap_rb_C s rb)) < unat(size_C (heap_rb_C s rb)) 
-                            \<and> (\<forall>i <  unat (size_C (heap_rb_C s rb)). is_valid_buffer_C s (ring_C (heap_rb_C s rb) +\<^sub>p i))"
+definition c_rb_valid :: " lifted_globals \<Rightarrow> rb_C ptr \<Rightarrow> bool"
+  where "c_rb_valid s rb \<longleftrightarrow> c_rb_valid_is_valid s rb 
+                            \<and> c_rb_valid_size s rb  \<and> c_rb_valid_head s rb
+                            \<and> c_rb_valid_tail s rb  \<and> c_rb_valid_ring s rb"
 
 
+(* ==================================================================================== *)
+subsection \<open>State Lifting\<close>
+(* ==================================================================================== *)
+
+
+text \<open>
+  We now define the lifting function which converts the \verb+rb_C+ object into a
+  \verb+CleanQ_RB+ record. We use the \verb+buffer_C+ representation for the buffer 
+  descriptor type in the record.
+\<close>
+
+(* 
 definition
   the_rb :: "lifted_globals \<Rightarrow> buffer_C ptr \<Rightarrow> nat \<Rightarrow> buffer"
   where
   "the_rb s b i =  \<lparr> base = unat (offset_C (heap_buffer_C s (b  +\<^sub>p i))),
                      length = unat (length_C (heap_buffer_C s (b  +\<^sub>p i))) \<rparr>"
+*)
 
+(* XXX: Should the ring here be taking the size of the ring buffer into account? 
+      ring = \<lambda>i. (if i <  size_C (heap_rb_C s rb) then heap_buffer_C s ((ring_C (heap_rb_C s rb))  +\<^sub>p i)),
+*)
 definition rb_C_to_CleanQ_RB :: "lifted_globals \<Rightarrow> rb_C ptr \<Rightarrow> buffer_C  CleanQ_RB"
-  where "rb_C_to_CleanQ_RB s rb = \<lparr>  ring = \<lambda>i. heap_buffer_C s ((ring_C (heap_rb_C s rb))  +\<^sub>p i),
-                                     head =  unat (head_C (heap_rb_C s rb)), 
-                                     tail =  unat (tail_C (heap_rb_C s rb)),
-                                     size =  unat (size_C (heap_rb_C s rb)) \<rparr>"
-
-lemma c_can_deq:
-  fixes rb :: "rb_C ptr"
-  shows 
-  "\<lbrace> \<lambda>s. rb_valid_c s rb  \<rbrace>
-   rb_can_deq_c_fun rb
-   \<lbrace> \<lambda> r s. r = (if rb_can_deq (rb_C_to_CleanQ_RB s rb) then 1 else 0) \<rbrace>!"
-  apply(subst rb_can_deq_c_fun_def)
-  apply(wp)
-  unfolding rb_can_deq_def rb_empty_def rb_C_to_CleanQ_RB_def rb_valid_c_def
-  by(auto)
-
-
-  
-
-
-
-lemma c_can_enq:
-  fixes rb :: "rb_C ptr"
-  shows 
-  "\<lbrace> \<lambda>s. rb_valid_c s rb  \<rbrace>
-   rb_can_enq_c_fun rb
-   \<lbrace> \<lambda> r s. r = (if rb_can_enq (rb_C_to_CleanQ_RB s rb) then 1 else 0) \<rbrace>!"
-  apply(subst rb_can_enq_c_fun_def)
-  apply(wp) 
-  unfolding rb_can_enq_def rb_full_def rb_C_to_CleanQ_RB_def 
-  apply(simp add:rb_valid_c_def)
-  using unat_64word_lt_succ_leq word_less_nat_alt by fastforce
-
-
-lemma c_rb_enq:
-  fixes rb :: "rb_C ptr" and b :: buffer_C
-  assumes full: "rb_can_enq_c_fun rb =  return (0)"
-  shows 
-  "\<lbrace> \<lambda>s. rb_valid_c s rb \<and> s0 = s  \<rbrace>
-   rb_enq_c_fun rb b
-   \<lbrace> \<lambda> r s. r \<noteq> 0 \<rbrace>!"
-   apply(subst rb_enq_c_fun_def)
-  apply(wp)
-   apply(auto)
-  apply(subst full)
-  apply(wp)
-  apply(simp)
-  done
- 
-
-  
-lemma c_rb_enq2:
-  fixes rb :: "rb_C ptr" and b :: buffer_C and s0 :: lifted_globals
-  assumes full: "rb_can_enq_c_fun rb =  return (0)"
-  shows "
-   \<lbrace> \<lambda>s. rb_valid_c s rb \<and> s0 = s  \<rbrace>
-   rb_enq_c_fun rb b
-   \<lbrace> \<lambda> r s. r \<noteq> 0 \<and> s = s0 \<rbrace>!"
-   apply(simp add:rb_enq_c_fun_def)
-   apply(wp, simp add:full)+
-   done
-
-  
-
-
-
-
-lemma c_rb_enq4:
-  fixes rb :: "rb_C ptr" and b :: buffer_C and s0 :: lifted_globals
-  assumes space: "rb_can_enq_c_fun rb =  return (1)" and prev: "rb0 = rb_C_to_CleanQ_RB s rb"
-  shows "
-   \<lbrace> \<lambda>s. rb_valid_c s rb \<and> s0 = s  \<rbrace>
-   rb_enq_c_fun rb b
-   \<lbrace> \<lambda> r s. r =0 \<and> s \<noteq> s0 \<and> rb_C_to_CleanQ_RB s rb = rb_enq b rb0  \<rbrace>!"
-  apply(simp add:rb_enq_c_fun_def)
-  apply(wp)
-  apply(simp add:space)
-   apply(wp_once)
-  apply(auto)
-      prefer 5 apply(simp add:rb_valid_c_def)
-  prefer 4 apply(simp add:rb_valid_c_def)
-  apply (metis int_unat)
-    prefer 3 apply(simp add:rb_valid_c_def)
-   prefer 2 apply(simp add:rb_enq_def rb_C_to_CleanQ_RB_def prev) 
-  apply(simp add:rb_incr_head_def rb_write_def) apply(auto)
-  
-  sorry
-
-
-
-
-(* ==================================================================================== *)
-subsection \<open>Enqueue Operation\<close>
-(* ==================================================================================== *)
+  where "rb_C_to_CleanQ_RB s rb = \<lparr> 
+                  ring = \<lambda>i. heap_buffer_C s (ring_C (heap_rb_C s rb)  +\<^sub>p i),
+                  head =  unat (head_C (heap_rb_C s rb)), 
+                  tail =  unat (tail_C (heap_rb_C s rb)),
+                  size =  unat (size_C (heap_rb_C s rb)) \<rparr>"
 
 text \<open>
-  For the enqueue operation, we can show that the operation preserves the size of the
-  ring buffer, and the tail pointer.
-\<close>
-
-lemma c_rb_enq_preserves_size :
-  fixes rb :: "rb_C ptr"
-  shows
-  "\<lbrace> \<lambda>s. rb_valid_c s rb \<and> s0 = s \<rbrace>
-   rb_enq_c_fun rb b
-   \<lbrace> \<lambda> r s. size_C (heap_rb_C s rb) = size_C (heap_rb_C s0 rb)  \<rbrace>!"
-   apply(simp add:rb_enq_c_fun_def)
-  apply(wp_once)+
-  apply(auto simp:rb_can_enq_c_fun_def)
-  apply(wp_once)+
-  apply(auto simp:rb_valid_c_def) 
-  apply (metis int_unat)
-  apply (simp add: unat_64word_leq_lt_lt Suc_leI word_less_nat_alt)
-  done
-
-lemma c_rb_enq_preserves_size2 :
-  fixes rb :: "rb_C ptr"
-  shows
-  "\<lbrace> \<lambda>s. rb_valid_c s rb \<and> size_C (heap_rb_C s rb) = k \<rbrace>
-   rb_enq_c_fun rb b
-   \<lbrace> \<lambda> r s. size_C (heap_rb_C s rb) = k  \<rbrace>!"
-   apply(simp add:rb_enq_c_fun_def)
-  apply(wp_once)+
-  apply(auto simp:rb_can_enq_c_fun_def)
-  apply(wp_once)+
-  apply(auto simp:rb_valid_c_def) 
-  apply (metis int_unat)
-  apply (simp add: unat_64word_leq_lt_lt Suc_leI word_less_nat_alt)
-  done
-
-
-lemma c_rb_enq_preserves_tail :
-  fixes rb :: "rb_C ptr"
-  shows
-  "\<lbrace> \<lambda>s. rb_valid_c s rb \<and> s0 = s \<rbrace>
-   rb_enq_c_fun rb b
-   \<lbrace> \<lambda> r s. tail_C (heap_rb_C s rb) = tail_C (heap_rb_C s0 rb)  \<rbrace>!"
-   apply(simp add:rb_enq_c_fun_def)
-  apply(wp_once)+
-  apply(auto simp:rb_can_enq_c_fun_def)
-  apply(wp_once)+
-  apply(auto simp:rb_valid_c_def) 
-  apply (metis int_unat)
-  apply (simp add: unat_64word_leq_lt_lt Suc_leI word_less_nat_alt)
-  done
-
-lemma c_rb_enq_preserves_tail2 :
-  fixes rb :: "rb_C ptr"
-  shows
-  "\<lbrace> \<lambda>s. rb_valid_c s rb \<and>  tail_C (heap_rb_C s rb) = k \<rbrace>
-   rb_enq_c_fun rb b
-   \<lbrace> \<lambda> r s.  tail_C (heap_rb_C s rb) = k  \<rbrace>!"
-   apply(simp add:rb_enq_c_fun_def)
-  apply(wp_once)+
-  apply(auto simp:rb_can_enq_c_fun_def)
-  apply(wp_once)+
-  apply(auto simp:rb_valid_c_def) 
-  apply (metis int_unat)
-  apply (simp add: unat_64word_leq_lt_lt Suc_leI word_less_nat_alt)
-  done
-
-
-text \<open>
-  If the queue is full, and the enqueue operation cannot put another buffer into
-  the ring, then the ring buffer remains in the same state. .
+  We can now show that if the C ringbuffer is valid, then the lifted state is also
+  satisfying the validity predicate of the \verb+CleanQ_RB+ model.
 \<close>
 
 
-lemma c_rb_enq_preserves_head :
-  fixes rb :: "rb_C ptr"
-  shows
-  "\<lbrace> \<lambda>s. rb_valid_c s rb \<and> s0 = s \<and> rb_can_enq_c_fun rb = return (0)  \<rbrace>
-   rb_enq_c_fun rb b
-   \<lbrace> \<lambda> r s. head_C (heap_rb_C s rb) = head_C (heap_rb_C s0 rb)  \<rbrace>!"
-   apply(simp add:rb_enq_c_fun_def)
-   apply(wp_once)+
-   apply(smt hoare_assume_preNF validNF_chain validNF_return)
-   done
-
-lemma c_rb_enq_preserves_head2 :
-  fixes rb :: "rb_C ptr"
-  shows
-  "\<lbrace> \<lambda>s. rb_valid_c s rb \<and> head_C (heap_rb_C s rb) = k \<and> rb_can_enq_c_fun rb = return (0) \<rbrace>
-   rb_enq_c_fun rb b
-   \<lbrace> \<lambda> r s. head_C (heap_rb_C s rb) = k \<rbrace>!"
-   apply(simp add:rb_enq_c_fun_def)
-   apply(wp_once)+
-   apply(smt hoare_assume_preNF validNF_chain validNF_return)
-   done
-
-lemma c_rb_enq_preserves_ring :
-  fixes rb :: "rb_C ptr"
-  shows
-  "\<lbrace> \<lambda>s. rb_valid_c s rb \<and> s0 = s \<and> rb_can_enq_c_fun rb = return (0)  \<rbrace>
-   rb_enq_c_fun rb b
-   \<lbrace> \<lambda> r s. ring_C (heap_rb_C s rb) = ring_C (heap_rb_C s0 rb)  \<rbrace>!"
-   apply(simp add:rb_enq_c_fun_def)
-   apply(wp_once)+
-   apply(smt hoare_assume_preNF validNF_chain validNF_return)
-   done
-
-
-lemma c_rb_enq_preserves_ring2 :
-  fixes rb :: "rb_C ptr"
-  shows
-  "\<lbrace> \<lambda>s. rb_valid_c s rb \<and> ring_C (heap_rb_C s rb) = k \<and> rb_can_enq_c_fun rb = return (0) \<rbrace>
-   rb_enq_c_fun rb b
-   \<lbrace> \<lambda> r s. ring_C (heap_rb_C s rb) = k  \<rbrace>!"
-   apply(simp add:rb_enq_c_fun_def)
-   apply(wp_once)+
-   apply(smt hoare_assume_preNF validNF_chain validNF_return)
-   done
-
-text \<open>
-  In fact, if the ring buffer is full, then the state is not altered at all.
-\<close>
-
-lemma c_rb_enq_full_preserves_state:
-  fixes rb :: "rb_C ptr" and b :: buffer_C
-  shows "
-   \<lbrace> \<lambda>s. rb_valid_c s rb \<and> s0 = s \<and> rb_can_enq_c_fun rb =  return (0)  \<rbrace>
-   rb_enq_c_fun rb b
-   \<lbrace> \<lambda> r s. r \<noteq> 0 \<and> s = s0 \<rbrace>!"
-   apply(simp add:rb_enq_c_fun_def)
-  apply(wp_once)+
-  apply(simp)
-  apply (smt hoare_assume_preNF validNF_chain validNF_return)
-  done
-
+lemma "c_rb_valid s rb \<longrightarrow> rb_valid (rb_C_to_CleanQ_RB s rb)"
+  unfolding c_rb_valid_def rb_valid_def rb_C_to_CleanQ_RB_def
+  using unat_word_lt by fastforce
 
 
 (* ==================================================================================== *)
 subsection \<open>Dequeue Operation\<close>
 (* ==================================================================================== *)
+
+text \<open>
+  Whether or not the dequeue operation performs the update, depends on whether the
+  the ring buffer is empty or not. We first show that the \verb+rb_can_deq+ function in 
+  C produces the same result as the corresponding definition in the \verb+CleanQ_RB+ 
+  model.
+\<close>
+
+lemma c_can_deq:
+  "\<lbrace> \<lambda>s. c_rb_valid s rb  \<rbrace>
+   rb_can_deq_c_fun rb
+   \<lbrace> \<lambda> r s. to_bool r =  rb_can_deq (rb_C_to_CleanQ_RB s rb) \<rbrace>!"
+  apply(subst rb_can_deq_c_fun_def)
+  apply(wp)
+  apply (simp add:rb_can_deq_def rb_empty_def rb_C_to_CleanQ_RB_def c_rb_valid_def)
+  done
+
+
+lemma c_can_deq_return_values:
+  "\<lbrace> \<lambda>s. is_valid_rb_C s rb  \<rbrace>
+   rb_can_deq_c_fun rb 
+   \<lbrace> \<lambda> r s. r =  0 \<or> r = 1  \<rbrace>!"
+  unfolding rb_can_deq_c_fun_def
+  by(wp, auto)  
 
 text \<open>
   For the dequeue operation, we can show that the operation preserves the size of the
@@ -424,60 +390,57 @@ text \<open>
 lemma c_rb_deq_preserves_size :
   fixes rb :: "rb_C ptr"
   shows
-  "\<lbrace> \<lambda>s. rb_valid_c s rb \<and> s0 = s \<and>  is_valid_buffer_C s b \<rbrace>
+  "\<And>s0. \<lbrace> \<lambda>s. c_rb_valid s rb \<and> s0 = s \<and> is_valid_buffer_C s b \<rbrace>
    rb_deq_c_fun rb b
    \<lbrace> \<lambda> r s. size_C (heap_rb_C s rb) = size_C (heap_rb_C s0 rb) \<rbrace>!"
    apply(simp add:rb_deq_c_fun_def)
   apply(wp_once)+
   apply(auto simp:rb_can_deq_c_fun_def)
   apply(wp_once)+
-  apply(auto simp:rb_valid_c_def) 
-  apply (metis int_unat)
-  done
+  apply(simp add:c_rb_valid_def)
+  by (metis less_imp_le uint_0_iff uint_lt_0 unat_gt_0  word_less_def)
+  
 
 
 lemma c_rb_deq_preserves_size2 :
   fixes rb :: "rb_C ptr"
   shows
-  "\<lbrace> \<lambda>s. rb_valid_c s rb \<and> size_C (heap_rb_C s rb) = k  \<and>  is_valid_buffer_C s b \<rbrace>
+  "\<lbrace> \<lambda>s. c_rb_valid s rb \<and> size_C (heap_rb_C s rb) = k  \<and>  is_valid_buffer_C s b \<rbrace>
    rb_deq_c_fun rb b
    \<lbrace> \<lambda> r s. size_C (heap_rb_C s rb) = k  \<rbrace>!"
    apply(simp add:rb_deq_c_fun_def)
   apply(wp_once)+
   apply(auto simp:rb_can_deq_c_fun_def)
   apply(wp_once)+
-  apply(auto simp:rb_valid_c_def)  
-  apply (metis int_unat)
-  done
+  apply(simp add:c_rb_valid_def)
+  by (metis less_imp_le uint_0_iff uint_lt_0 unat_gt_0  word_less_def)
 
 
 lemma c_rb_deq_preserves_head :
   fixes rb :: "rb_C ptr"
   shows
-  "\<lbrace> \<lambda>s. rb_valid_c s rb \<and> s0 = s  \<and>  is_valid_buffer_C s b \<rbrace>
+  "\<lbrace> \<lambda>s. c_rb_valid s rb \<and> s0 = s  \<and>  is_valid_buffer_C s b \<rbrace>
    rb_deq_c_fun rb b
    \<lbrace> \<lambda> r s. head_C (heap_rb_C s rb) = head_C (heap_rb_C s0 rb)  \<rbrace>!"
    apply(simp add:rb_deq_c_fun_def)
   apply(wp_once)+
   apply(auto simp:rb_can_deq_c_fun_def)
   apply(wp_once)+
-  apply(auto simp:rb_valid_c_def) 
-  apply (metis int_unat)
-  done
+  apply(simp add:c_rb_valid_def)
+  by (metis less_imp_le uint_0_iff uint_lt_0 unat_gt_0  word_less_def)
 
 lemma c_rb_deq_preserves_head2 :
   fixes rb :: "rb_C ptr"
   shows
-  "\<lbrace> \<lambda>s. rb_valid_c s rb \<and>  head_C (heap_rb_C s rb) = k  \<and> is_valid_buffer_C s b \<rbrace>
+  "\<lbrace> \<lambda>s. c_rb_valid s rb \<and>  head_C (heap_rb_C s rb) = k  \<and> is_valid_buffer_C s b \<rbrace>
    rb_deq_c_fun rb b
    \<lbrace> \<lambda> r s.  head_C (heap_rb_C s rb) = k  \<rbrace>!"
-   apply(simp add:rb_deq_c_fun_def)
+  apply(simp add:rb_deq_c_fun_def)
   apply(wp_once)+
   apply(auto simp:rb_can_deq_c_fun_def)
   apply(wp_once)+
-  apply(auto simp:rb_valid_c_def)  
-  apply (metis int_unat)
-  done
+  apply(simp add:c_rb_valid_def)
+  by (metis less_imp_le uint_0_iff uint_lt_0 unat_gt_0  word_less_def)
 
 
 text \<open>
@@ -489,55 +452,384 @@ text \<open>
 lemma c_rb_deq_preserves_tail :
   fixes rb :: "rb_C ptr"
   shows
-  "\<lbrace> \<lambda>s. rb_valid_c s rb \<and> s0 = s \<and> rb_can_deq_c_fun rb = return (0)  \<and> is_valid_buffer_C s b \<rbrace>
+  "\<lbrace> \<lambda>s. c_rb_valid s rb \<and> s0 = s \<and> rb_can_deq_c_fun rb = return (0)  \<rbrace>
    rb_deq_c_fun rb b
    \<lbrace> \<lambda> r s. tail_C (heap_rb_C s rb) = tail_C (heap_rb_C s0 rb)  \<rbrace>!"
-   apply(simp add:rb_deq_c_fun_def)
-   apply(wp_once)+
-   apply(smt hoare_assume_preNF validNF_chain validNF_return)
-   done
+  apply(simp add:rb_deq_c_fun_def)
+  apply(wp_once)+
+  apply(smt hoare_assume_preNF validNF_chain validNF_return)
+  done
 
 lemma c_rb_deq_preserves_tail2 :
   fixes rb :: "rb_C ptr"
   shows
-  "\<lbrace> \<lambda>s. rb_valid_c s rb \<and> tail_C (heap_rb_C s rb) = k \<and> rb_can_deq_c_fun rb = return (0)  \<and> is_valid_buffer_C s b \<rbrace>
+  "\<lbrace> \<lambda>s. c_rb_valid s rb \<and> tail_C (heap_rb_C s rb) = k \<and> rb_can_deq_c_fun rb = return (0) \<rbrace>
    rb_deq_c_fun rb b
    \<lbrace> \<lambda> r s. tail_C (heap_rb_C s rb) = k \<rbrace>!"
-   apply(simp add:rb_deq_c_fun_def)
-   apply(wp_once)+
-   apply(smt hoare_assume_preNF validNF_chain validNF_return)
-   done
+  apply(simp add:rb_deq_c_fun_def)
+  apply(wp_once)+
+  apply(smt hoare_assume_preNF validNF_chain validNF_return)
+  done
+
+text \<open>
+  The dequeue operation does not change the ring at all
+\<close>
 
 lemma c_rb_deq_preserves_ring :
   fixes rb :: "rb_C ptr"
   shows
-  "\<lbrace> \<lambda>s. rb_valid_c s rb \<and> s0 = s \<and> rb_can_deq_c_fun rb = return (0) \<and> is_valid_buffer_C s b \<rbrace>
+  "\<lbrace> \<lambda>s. c_rb_valid s rb \<and> s0 = s \<and> is_valid_buffer_C s0 b  \<rbrace>
    rb_deq_c_fun rb b
    \<lbrace> \<lambda> r s. ring_C (heap_rb_C s rb) = ring_C (heap_rb_C s0 rb)  \<rbrace>!"
    apply(simp add:rb_deq_c_fun_def)
-   apply(wp_once)+
-   apply(smt hoare_assume_preNF validNF_chain validNF_return)
-   done
+  apply(wp_once)+
+  apply(simp add:rb_can_deq_c_fun_def)
+  apply(wp_once)+
+  apply(auto simp add:c_rb_valid_def)
+  using unat_word_lt apply fastforce
+  using word_le_def word_le_less_eq apply blast 
+  done
 
 lemma c_rb_deq_preserves_ring2 :
   fixes rb :: "rb_C ptr"
   shows
-  "\<lbrace> \<lambda>s. rb_valid_c s rb \<and> ring_C (heap_rb_C s rb) = k \<and> rb_can_deq_c_fun rb = return (0)  \<and> is_valid_buffer_C s b \<rbrace>
+  "\<lbrace> \<lambda>s. c_rb_valid s rb \<and> ring_C (heap_rb_C s rb) = k \<and> is_valid_buffer_C s b \<rbrace>
    rb_deq_c_fun rb b
    \<lbrace> \<lambda> r s. ring_C (heap_rb_C s rb) = k  \<rbrace>!"
    apply(simp add:rb_deq_c_fun_def)
-   apply(wp_once)+
-   apply(smt hoare_assume_preNF validNF_chain validNF_return)
-   done
+  apply(wp_once)+
+  apply(simp add:rb_can_deq_c_fun_def)
+  apply(wp_once)+
+  apply(auto simp add:c_rb_valid_def)
+  using unat_word_lt apply fastforce
+  using word_le_def word_le_less_eq apply blast 
+  done
+
+text \<open>
+  Also, the ring contents are not changed. 
+\<close>
+
+lemma c_rb_deq_preserves_ring_contents :
+  fixes rb :: "rb_C ptr"
+  shows
+  "\<lbrace> \<lambda>s. c_rb_valid s rb \<and> s0 = s \<and> is_valid_buffer_C s0 b 
+    \<and> (\<forall>i < size_C (heap_rb_C s rb).  (ring_C (heap_rb_C s rb)  +\<^sub>p uint i) \<noteq> b)   \<rbrace>
+   rb_deq_c_fun rb b
+   \<lbrace> \<lambda> r s. \<forall>i < size_C (heap_rb_C s rb). 
+        heap_buffer_C s (ring_C (heap_rb_C s rb)  +\<^sub>p uint i) = 
+        heap_buffer_C s0 (ring_C (heap_rb_C s0 rb) +\<^sub>p uint i)  \<rbrace>!"
+   apply(simp add:rb_deq_c_fun_def)
+  apply(wp_once)+
+  apply(simp add:rb_can_deq_c_fun_def)
+  apply(wp_once)+
+  apply(auto simp add:c_rb_valid_def)
+  using unat_word_lt apply fastforce
+  using word_le_def word_le_less_eq apply blast 
+  using unat_word_lt apply fastforce
+  using less_imp_le word_le_def apply blast
+  done
+
 
 text \<open>
   In fact, if the ring buffer is empty, then the state is not altered at all.
 \<close>
 
-lemma c_rb_deq_full_preserves_state:
+lemma c_rb_deq_empty_preserves_state:
   fixes rb :: "rb_C ptr" and b :: buffer_C
   shows "
-   \<lbrace> \<lambda>s. rb_valid_c s rb \<and> s0 = s \<and> rb_can_enq_c_fun rb =  return (0)  \<rbrace>
+   \<lbrace> \<lambda>s. c_rb_valid s rb \<and> s0 = s \<and> rb_can_enq_c_fun rb =  return (0)  \<rbrace>
+   rb_enq_c_fun rb b
+   \<lbrace> \<lambda> r s. r \<noteq> 0 \<and> s = s0 \<rbrace>!"
+   apply(simp add:rb_enq_c_fun_def)
+  apply(wp_once)+
+  apply(simp)
+  apply (smt hoare_assume_preNF validNF_chain validNF_return)
+  done
+
+text \<open>
+  We can show that the dequeue function preserves the valid predicate.
+\<close>
+
+lemma c_rb_deq_remains_valid:
+  fixes rb :: "rb_C ptr" 
+  shows "
+   \<lbrace> \<lambda>s. c_rb_valid s rb \<and> is_valid_buffer_C s b  \<rbrace>
+   rb_deq_c_fun rb b
+   \<lbrace> \<lambda> r s.  c_rb_valid s rb \<rbrace>!"
+  apply(simp add:rb_deq_c_fun_def)
+  apply(wp_once)+
+  apply(simp add:rb_can_deq_c_fun_def)
+  apply(wp_once)+
+  apply(simp add:c_rb_valid_def)
+  by (metis not_gr_zero not_less0 unat_0 word_le_def word_le_less_eq word_less_nat_alt 
+            word_mod_less_divisor)
+
+
+text \<open>
+  Lastly, we can show that the C implementation of the dequeue operation produces the 
+  same outcome as doing the abstraction operation.
+\<close>
+
+lemma c_rb_deq_state_update_head:
+"\<lbrace> \<lambda>s. c_rb_valid s rb \<and> s0 = s \<and> rb0 = rb_C_to_CleanQ_RB s rb  
+        \<and> is_valid_buffer_C s0 b  \<rbrace>
+   rb_deq_c_fun rb b
+ \<lbrace> \<lambda> r s. head (rb_C_to_CleanQ_RB s rb) = head (snd (rb_deq rb0)) \<rbrace>!"
+  unfolding rb_deq_c_fun_def
+  apply(wp_once)+
+  apply(simp add:rb_can_deq_c_fun_def)
+  apply(wp_once)+
+  apply(simp add:c_rb_valid_def rb_deq_equiv rb_deq_alt_def rb_C_to_CleanQ_RB_def)
+  using less_imp_le unat_1_0  word_le_def word_le_less_eq by blast
+ 
+  
+lemma c_rb_deq_state_update_tail:
+  "\<lbrace> \<lambda>s. c_rb_valid s rb \<and> s0 = s \<and> rb0 = rb_C_to_CleanQ_RB s rb   \<and> is_valid_buffer_C s0 b  \<rbrace>
+   rb_deq_c_fun rb b
+   \<lbrace> \<lambda> r s. (r = ERR_OK \<or> r = ERR_QUEUE_EMPTY) \<and>
+      (if r = ERR_OK then tail (rb_C_to_CleanQ_RB s rb) = tail (snd (rb_deq rb0)) 
+       else s = s0)  \<rbrace>!"
+  unfolding rb_deq_c_fun_def
+  apply(wp_once)+
+  apply(simp add:rb_can_deq_c_fun_def)
+  apply(wp_once)+
+  apply(simp add:c_rb_valid_def rb_deq_equiv rb_deq_alt_def rb_C_to_CleanQ_RB_def)
+  by (metis unat_1 unat_1_0 unat_32word_succ_mod unat_word_lt word_le_def word_le_less_eq)
+
+
+lemma c_rb_deq_state_update_size:
+  "\<lbrace> \<lambda>s. c_rb_valid s rb \<and> s0 = s 
+                \<and> rb0 = rb_C_to_CleanQ_RB s rb  \<and> is_valid_buffer_C s0 b  \<rbrace>
+   rb_deq_c_fun rb b
+   \<lbrace> \<lambda> r s.  (r = ERR_OK \<or> r = ERR_QUEUE_EMPTY) \<and>
+              size (rb_C_to_CleanQ_RB s rb) = size (snd (rb_deq rb0)) \<rbrace>!"
+  unfolding rb_deq_c_fun_def
+  apply(wp_once)+
+  apply(simp add:rb_can_deq_c_fun_def)
+  apply(wp_once)+
+  apply(simp add:c_rb_valid_def rb_deq_equiv rb_deq_alt_def rb_C_to_CleanQ_RB_def)
+  using less_imp_le unat_1_0  word_le_def word_le_less_eq by blast
+
+
+lemma foobar:
+  "ring (snd (rb_deq (rb_C_to_CleanQ_RB s rb))) = ring (rb_C_to_CleanQ_RB s rb)"
+  unfolding rb_C_to_CleanQ_RB_def
+  by(auto simp: rb_deq_equiv rb_deq_alt_def)
+
+lemma c_rb_deq_state_update_ring:
+  assumes notinring: "(\<forall>i \<le> uint (size_C (heap_rb_C s0 rb)). 
+                                     (ring_C (heap_rb_C s0 rb) +\<^sub>p i) \<noteq> b)"
+  shows "
+   \<lbrace> \<lambda>s. c_rb_valid s rb \<and> s0 = s  
+                \<and> rb0 = rb_C_to_CleanQ_RB s rb  \<and> is_valid_buffer_C s b  \<rbrace>
+   rb_deq_c_fun rb b
+   \<lbrace> \<lambda> r s. (r = ERR_OK \<or> r = ERR_QUEUE_EMPTY) \<and> 
+         (if r = ERR_OK then \<forall> i < uint (size_C (heap_rb_C s rb)). ring (rb_C_to_CleanQ_RB s rb) i = ring (snd (rb_deq rb0)) i
+         else s = s0)  \<rbrace>!"
+  unfolding rb_deq_c_fun_def
+  apply(wp_once)+
+  apply(simp add:rb_can_deq_c_fun_def)
+  apply(wp_once)+ 
+  apply(auto simp:c_rb_valid_def  rb_deq_equiv rb_deq_alt_def)
+  prefer 3 using word_le_def word_le_less_eq apply blast
+   prefer 2 using unat_word_lt apply fastforce
+  unfolding rb_C_to_CleanQ_RB_def using notinring by(auto)
+ 
+
+lemma c_rb_deq_correct:
+  assumes notinring: "(\<forall>i \<le> uint (size_C (heap_rb_C s0 rb)). 
+                                     (ring_C (heap_rb_C s0 rb) +\<^sub>p i) \<noteq> b)"
+  shows "
+   \<lbrace> \<lambda>s. c_rb_valid s rb \<and> s0 = s  \<and> rb0 = rb_C_to_CleanQ_RB s rb \<and>  is_valid_buffer_C s0 b  \<rbrace>
+   rb_deq_c_fun rb b
+   \<lbrace> \<lambda> r s. (r = ERR_OK \<or> r = ERR_QUEUE_EMPTY) \<and> 
+        (if r = ERR_OK then rb_C_to_CleanQ_RB s rb = snd (rb_deq rb0) else s = s0)
+    \<rbrace>!"
+  (* \<and> heap_buffer_C s b = fst (rb_deq rb0)*)
+
+    unfolding rb_deq_c_fun_def
+  apply(wp_once)+
+  apply(simp add:rb_can_deq_c_fun_def)
+  apply(wp_once)+ 
+  apply(auto simp:c_rb_valid_def  rb_deq_equiv rb_deq_alt_def)
+  prefer 3 using word_le_def word_le_less_eq apply blast
+     prefer 2 using unat_word_lt apply fastforce
+    unfolding rb_C_to_CleanQ_RB_def using notinring 
+
+    (* XXX: can't show it like this, because we have to show that deq doesn't 
+            change the ring, there is a possibility to dequeue into the ring again. 
+            as deq takes a buffer pointer to return the value *)
+    oops
+  
+
+
+
+(* ==================================================================================== *)
+subsection \<open>Enqueue Operation\<close>
+(* ==================================================================================== *)
+
+text \<open>
+  Whether or not the enqueue operation performs the update, depends on whether the
+  the ring buffer is full or not. We first show that the \verb+rb_can_enq+ function in 
+  C produces the same result as the corresponding definition in the \verb+CleanQ_RB+ 
+  model.
+\<close>
+
+lemma c_can_enq:
+  fixes rb :: "rb_C ptr"
+  shows 
+  "\<lbrace> \<lambda>s. c_rb_valid s rb  \<rbrace>
+   rb_can_enq_c_fun rb
+   \<lbrace> \<lambda> r s. to_bool r =  rb_can_enq (rb_C_to_CleanQ_RB s rb) \<rbrace>!"
+  apply(subst rb_can_enq_c_fun_def)
+  apply(wp, simp add:rb_can_enq_def rb_full_def rb_C_to_CleanQ_RB_def c_rb_valid_def)
+  using Suc_le_eq unat_32word_leq_lt_lt unat_word_lt by fastforce
+
+
+lemma c_can_enq_return_values:
+  "\<lbrace> \<lambda>s. c_rb_valid s rb  \<rbrace>
+   rb_can_enq_c_fun rb 
+   \<lbrace> \<lambda> r s. r =  0 \<or> r = 1  \<rbrace>!"
+  unfolding rb_can_enq_c_fun_def
+  apply(wp, simp)
+  using c_rb_valid_def unat_32word_leq_lt_lt unat_gt_0 by fastforce
+
+
+text \<open>
+  For the enqueue operation, we can show that the operation preserves the size of the
+  ring buffer, and the tail pointer.
+\<close>
+
+lemma c_rb_enq_preserves_size :
+  fixes rb :: "rb_C ptr"
+  shows
+  "\<lbrace> \<lambda>s. c_rb_valid s rb \<and> s0 = s \<rbrace>
+   rb_enq_c_fun rb b
+   \<lbrace> \<lambda> r s. size_C (heap_rb_C s rb) = size_C (heap_rb_C s0 rb)  \<rbrace>!"
+  apply(simp add:rb_enq_c_fun_def)
+  apply(wp_once)+
+  apply(auto simp:rb_can_enq_c_fun_def)
+  apply(wp_once)+
+  apply(simp add:c_rb_valid_def unat_word_leq word_less_nat_alt) 
+  by (meson INT_MIN_MAX_lemmas(12) Suc_leI le_eq_less_or_eq less_le_trans un_ui_le)
+  
+
+lemma c_rb_enq_preserves_size2 :
+  fixes rb :: "rb_C ptr"
+  shows
+  "\<lbrace> \<lambda>s. c_rb_valid s rb \<and> size_C (heap_rb_C s rb) = k \<rbrace>
+   rb_enq_c_fun rb b
+   \<lbrace> \<lambda> r s. size_C (heap_rb_C s rb) = k  \<rbrace>!"
+   apply(simp add:rb_enq_c_fun_def)
+  apply(wp_once)+
+  apply(auto simp:rb_can_enq_c_fun_def)
+  apply(wp_once)+
+  apply(simp add:c_rb_valid_def unat_word_leq word_less_nat_alt) 
+  by (meson INT_MIN_MAX_lemmas(12) Suc_le_eq less_imp_le_nat less_le_trans un_ui_le)
+
+
+lemma c_rb_enq_preserves_tail :
+  fixes rb :: "rb_C ptr"
+  shows
+  "\<lbrace> \<lambda>s. c_rb_valid s rb \<and> s0 = s \<rbrace>
+   rb_enq_c_fun rb b
+   \<lbrace> \<lambda> r s. tail_C (heap_rb_C s rb) = tail_C (heap_rb_C s0 rb)  \<rbrace>!"
+   apply(simp add:rb_enq_c_fun_def)
+  apply(wp_once)+
+  apply(auto simp:rb_can_enq_c_fun_def)
+  apply(wp_once)+
+  apply(simp add:c_rb_valid_def word_less_nat_alt) 
+  by (meson INT_MIN_MAX_lemmas(12) Suc_leI le_eq_less_or_eq less_le_trans un_ui_le)
+
+lemma c_rb_enq_preserves_tail2 :
+  fixes rb :: "rb_C ptr"
+  shows
+  "\<lbrace> \<lambda>s. c_rb_valid s rb \<and>  tail_C (heap_rb_C s rb) = k \<rbrace>
+   rb_enq_c_fun rb b
+   \<lbrace> \<lambda> r s.  tail_C (heap_rb_C s rb) = k  \<rbrace>!"
+   apply(simp add:rb_enq_c_fun_def)
+  apply(wp_once)+
+  apply(auto simp:rb_can_enq_c_fun_def)
+  apply(wp_once)+
+  apply(simp add:c_rb_valid_def word_less_nat_alt) 
+  by (meson INT_MIN_MAX_lemmas(12) Suc_le_eq less_imp_le_nat less_le_trans un_ui_le)
+
+
+text \<open>
+  If the queue is full, and the enqueue operation cannot put another buffer into
+  the ring, then the ring buffer remains in the same state. .
+\<close>
+
+
+lemma c_rb_enq_preserves_head :
+  fixes rb :: "rb_C ptr"
+  shows
+  "\<lbrace> \<lambda>s. c_rb_valid s rb \<and> s0 = s \<and> rb_can_enq_c_fun rb = return (0)  \<rbrace>
+   rb_enq_c_fun rb b
+   \<lbrace> \<lambda> r s. head_C (heap_rb_C s rb) = head_C (heap_rb_C s0 rb)  \<rbrace>!"
+   apply(simp add:rb_enq_c_fun_def)
+   apply(wp_once)+
+   apply(smt hoare_assume_preNF validNF_chain validNF_return)
+   done
+
+lemma c_rb_enq_preserves_head2 :
+  fixes rb :: "rb_C ptr"
+  shows
+  "\<lbrace> \<lambda>s. c_rb_valid s rb \<and> head_C (heap_rb_C s rb) = k \<and> rb_can_enq_c_fun rb = return (0) \<rbrace>
+   rb_enq_c_fun rb b
+   \<lbrace> \<lambda> r s. head_C (heap_rb_C s rb) = k \<rbrace>!"
+   apply(simp add:rb_enq_c_fun_def)
+   apply(wp_once)+
+   apply(smt hoare_assume_preNF validNF_chain validNF_return)
+   done
+ 
+lemma c_rb_enq_preserves_ring :
+  fixes rb :: "rb_C ptr"
+  shows
+  "\<lbrace> \<lambda>s. c_rb_valid s rb \<and> s0 = s \<and> rb_can_enq_c_fun rb = return (0)  \<rbrace>
+   rb_enq_c_fun rb b
+   \<lbrace> \<lambda> r s. ring_C (heap_rb_C s rb) = ring_C (heap_rb_C s0 rb)  \<rbrace>!"
+   apply(simp add:rb_enq_c_fun_def)
+   apply(wp_once)+
+   apply(smt hoare_assume_preNF validNF_chain validNF_return)
+   done
+
+
+lemma c_rb_enq_preserves_ring2 :
+  fixes rb :: "rb_C ptr"
+  shows
+  "\<lbrace> \<lambda>s. c_rb_valid s rb \<and> ring_C (heap_rb_C s rb) = k \<and> rb_can_enq_c_fun rb = return (0) \<rbrace>
+   rb_enq_c_fun rb b
+   \<lbrace> \<lambda> r s. ring_C (heap_rb_C s rb) = k  \<rbrace>!"
+   apply(simp add:rb_enq_c_fun_def)
+   apply(wp_once)+
+   apply(smt hoare_assume_preNF validNF_chain validNF_return)
+   done
+
+text \<open>
+  Also, the ring contents are not changed, if we're full
+\<close>
+
+lemma c_rb_enq_full_preserves_ring_contents :
+  fixes rb :: "rb_C ptr"
+  shows
+  "\<lbrace> \<lambda>s. c_rb_valid s rb \<and> s0 = s \<and> rb_can_enq_c_fun rb = return (0) \<rbrace>
+   rb_enq_c_fun rb b
+   \<lbrace> \<lambda> r s. heap_buffer_C s (ring_C (heap_rb_C s rb)  +\<^sub>p uint i) = 
+            heap_buffer_C s0 (ring_C (heap_rb_C s0 rb) +\<^sub>p uint i)  \<rbrace>!"
+  apply(simp add:rb_enq_c_fun_def)
+  apply(wp_once)+
+  by(smt hoare_assume_preNF validNF_chain validNF_return)
+
+
+text \<open>
+  In fact, if the ring buffer is full, then the state is not altered at all.
+\<close>
+
+lemma c_rb_enq_full_preserves_state:
+  fixes rb :: "rb_C ptr" and b :: buffer_C
+  shows "
+   \<lbrace> \<lambda>s. c_rb_valid s rb \<and> s0 = s \<and> rb_can_enq_c_fun rb =  return (0)  \<rbrace>
    rb_enq_c_fun rb b
    \<lbrace> \<lambda> r s. r \<noteq> 0 \<and> s = s0 \<rbrace>!"
    apply(simp add:rb_enq_c_fun_def)
@@ -547,7 +839,336 @@ lemma c_rb_deq_full_preserves_state:
   done
 
 
+text \<open>
+  We can show that the enqueue function preserves the valid predicate.
+\<close>
 
+lemma c_rb_enq_remains_valid:
+  fixes rb :: "rb_C ptr" and b :: buffer_C
+  shows "
+   \<lbrace> \<lambda>s. c_rb_valid s rb  \<rbrace>
+   rb_enq_c_fun rb b
+   \<lbrace> \<lambda> r s.  c_rb_valid s rb \<rbrace>!"
+  apply(simp add:rb_enq_c_fun_def)
+  apply(wp_once)+
+  apply(simp add:rb_can_enq_c_fun_def)
+  apply(wp_once)+
+  apply(simp add:c_rb_valid_def )
+  by (meson INT_MIN_MAX_lemmas(12) less_eq_Suc_le less_trans not_less unat_1_0 
+            unat_32word_leq_lt_lt word_le_less_eq word_less_1 word_less_def 
+            word_mod_less_divisor)
+
+  
+text \<open>
+  Lastly, we can show that the C implementation of the enqueue operation produces the 
+  same outcome as doing the abstraction operation.
+\<close>
+
+lemma c_rb_enq_state_update_head:
+  "\<lbrace> \<lambda>s. c_rb_valid s rb \<and> s0 = s  \<and> rb0 = rb_C_to_CleanQ_RB s rb   \<rbrace>
+   rb_enq_c_fun rb b
+   \<lbrace> \<lambda> r s. (r = ERR_OK \<or> r = ERR_QUEUE_FULL) \<and> 
+         (if r = ERR_OK then head (rb_C_to_CleanQ_RB s rb) = head (rb_enq b rb0)
+         else s = s0) \<rbrace>!"
+  unfolding rb_enq_c_fun_def  rb_C_to_CleanQ_RB_def rb_enq_equiv rb_enq_alt_def
+  apply(wp_once)+
+  apply(simp add:rb_can_enq_c_fun_def)
+  apply(wp_once)+
+  apply(auto simp:c_rb_valid_def unat_32word_succ_mod Suc_leI unat_32word_leq_lt_lt 
+                  word_less_nat_alt)
+  using word_le_def word_le_less_eq word_less_nat_alt by blast
+
+lemma c_rb_enq_state_update_tail:
+  "\<lbrace> \<lambda>s. c_rb_valid s rb \<and> s0 = s  \<and> rb0 = rb_C_to_CleanQ_RB s rb   \<rbrace>
+   rb_enq_c_fun rb b
+   \<lbrace> \<lambda> r s.  (r = ERR_OK \<or> r = ERR_QUEUE_FULL) \<and> 
+       tail (rb_C_to_CleanQ_RB s rb) = tail (rb_enq b rb0)  \<rbrace>!"
+  unfolding rb_enq_c_fun_def rb_C_to_CleanQ_RB_def
+  apply(wp_once)+
+  apply(auto simp:rb_can_enq_c_fun_def)
+  apply(wp_once)+
+  apply(auto simp: rb_enq_alt_def rb_enq_equiv c_rb_valid_def word_less_nat_alt Suc_leI 
+                   unat_32word_leq_lt_lt)
+  by (meson le_eq_less_or_eq un_ui_le)
+
+lemma c_rb_enq_state_update_size:
+  "\<lbrace> \<lambda>s. c_rb_valid s rb \<and> s0 = s  \<and> rb0 = rb_C_to_CleanQ_RB s rb   \<rbrace>
+   rb_enq_c_fun rb b
+   \<lbrace> \<lambda> r s.  (r = ERR_OK \<or> r = ERR_QUEUE_FULL) \<and> 
+       size (rb_C_to_CleanQ_RB s rb) = size (rb_enq b rb0)  \<rbrace>!"
+  unfolding rb_enq_c_fun_def rb_C_to_CleanQ_RB_def
+  apply(wp_once)+
+  apply(auto simp:rb_can_enq_c_fun_def)
+  apply(wp_once)+
+  apply(auto simp: rb_enq_alt_def rb_enq_equiv c_rb_valid_def word_less_nat_alt Suc_leI 
+                   unat_32word_leq_lt_lt)
+  by (meson le_eq_less_or_eq un_ui_le)
+  
+
+
+lemma c_ring_ptr_different:
+assumes neq: "x \<noteq> unat (head_C (heap_rb_C s0 rb)) \<and> x < unat (size_C (heap_rb_C s0 rb))" 
+    and valid: "c_rb_valid s0 rb"
+  shows "ring_C (heap_rb_C s0 rb) +\<^sub>p int x \<noteq> ring_C (heap_rb_C s0 rb) +\<^sub>p uint (head_C (heap_rb_C s0 rb))"
+proof-
+  have sizelimit:
+    "(size_C (heap_rb_C s0 rb)) \<le> 0xffffffff"
+    by (metis word_and_le1 word_and_max_simps(3))
+
+  have unatsizelimit:
+    "unat (size_C (heap_rb_C s0 rb)) \<le> 0xffffffff"
+    using sizelimit UINT_MAX_def by auto
+
+  have head_leq_size:
+     "unat (head_C (heap_rb_C s0 rb)) < unat (size_C (heap_rb_C s0 rb))"
+    using valid unfolding c_rb_valid_def
+    using unat_word_lt by blast
+   
+  have inrangex: 
+    "x * unat(0x40::64 word) \<le> unat addrlimit"
+    using neq unatsizelimit by(auto)
+
+  have inrangey: 
+    "unat (head_C (heap_rb_C s0 rb)) * unat (0x40::64 word) \<le> unat  addrlimit"
+     using  unatsizelimit head_leq_size by(auto)
+
+  have ineq:
+    "of_nat x * (0x40::ulong_t) \<noteq> of_int (uint (head_C (heap_rb_C s0 rb))) * (0x40::ulong_t)"
+    proof -
+      have f1: "\<forall>w n. of_int (int n) * (w::64 word) = of_int (int (n * unat w))"
+        by simp
+      have "unat (head_C (heap_rb_C s0 rb)) * unat (0x40::64 word) \<noteq> x * unat (0x40::64 word)"
+    using neq by auto
+    then have "(of_int (int x)::64 word) * 0x40 \<noteq> of_int (int (unat (head_C (heap_rb_C s0 rb)))) * 0x40"
+    using f1 by (metis (no_types) inrangex inrangey le_unat_uoi of_int_of_nat_eq)
+    then show ?thesis
+    by (simp add: int_unat)
+    qed
+
+  thus ?thesis unfolding ptr_add_def
+    by(auto)
+qed
+
+lemma c_rb_enq_state_update_ring_other:
+assumes neq: "x \<noteq> unat (head_C (heap_rb_C s0 rb)) \<and> x < unat (size_C (heap_rb_C s0 rb))"
+    and valid: "c_rb_valid s0 rb"
+    and supd: "s = heap_buffer_C_update 
+                          (\<lambda>a. a(ring_C (heap_rb_C s0 rb) 
+                                +\<^sub>p uint (head_C (heap_rb_C s0 rb)) := b)) s0"
+  shows "heap_buffer_C s (ring_C (heap_rb_C s rb) +\<^sub>p int x)
+        = heap_buffer_C s0 (ring_C (heap_rb_C s0 rb) +\<^sub>p int x)"
+  apply(subst supd)+ 
+  using neq valid unfolding c_rb_valid_def apply(simp)
+  using valid unfolding c_rb_valid_def 
+  by (simp add: CleanQ_SimpleQ.c_ring_ptr_different valid)
+
+
+lemma c_rb_enq_state_update_ring_head:
+  assumes eq: "x = unat (head_C (heap_rb_C s0 rb))"
+     and supd: "s = heap_buffer_C_update 
+                        (\<lambda>a. a(ring_C (heap_rb_C s0 rb)
+                               +\<^sub>p uint (head_C (heap_rb_C s0 rb)) := b)) s0"
+  shows "heap_buffer_C s (ring_C (heap_rb_C s rb) +\<^sub>p int x) = b"
+  using eq  by (simp add: int_unat supd)
+
+lemma c_rb_enq_state_ring_lifted_head:
+  assumes eq:  "x = unat (head_C (heap_rb_C s rb))"
+    shows  "ring (rb_enq b (rb_C_to_CleanQ_RB s rb)) x = b"
+  unfolding rb_C_to_CleanQ_RB_def rb_enq_alt_def rb_enq_equiv
+  using eq by(auto)
+
+lemma c_rb_enq_state_ring_lifted_other:
+  assumes eq:  "x \<noteq> unat (head_C (heap_rb_C s rb))"
+    shows  "ring (rb_enq b (rb_C_to_CleanQ_RB s rb)) x = ring (rb_C_to_CleanQ_RB s rb) x"
+  unfolding rb_C_to_CleanQ_RB_def rb_enq_alt_def rb_enq_equiv
+  using eq by(auto)
+
+lemma c_rb_enq_state_ring_head:
+  assumes eq:  "x = unat (head_C (heap_rb_C s0 rb))" 
+     and supd: "s = heap_buffer_C_update 
+                        (\<lambda>a. a(ring_C (heap_rb_C s0 rb)
+                                         +\<^sub>p uint (head_C (heap_rb_C s0 rb)) := b)) s0"
+     and hupd: "s1 = heap_rb_C_update
+                        (\<lambda>a. a(rb := head_C_update (\<lambda>a. 
+                              (a + (1)) mod size_C (heap_rb_C s0 rb)) (a rb))) s"
+   shows "ring (rb_C_to_CleanQ_RB s1 rb) x = b"
+   apply(auto simp:rb_C_to_CleanQ_RB_def)
+   unfolding rb_C_to_CleanQ_RB_def using eq by(auto simp:supd hupd int_unat)
+  
+
+lemma c_rb_enq_state_update_ring:
+  fixes rb :: "rb_C ptr" and b :: buffer_C
+  assumes notfull: " rb_can_enq_c_fun rb = return (1) "
+  shows "
+   \<lbrace> \<lambda>s. rb_can_enq_c_fun rb = return (1) \<and> (c_rb_valid s rb \<and> s0 = s 
+                \<and> rb0 = rb_C_to_CleanQ_RB s rb)   \<rbrace>
+   rb_enq_c_fun rb b
+   \<lbrace> \<lambda> r s. \<forall>i < size rb0. ring (rb_C_to_CleanQ_RB s rb) i = ring (rb_enq b rb0) i \<rbrace>!"
+  unfolding rb_enq_c_fun_def  rb_C_to_CleanQ_RB_def rb_enq_equiv rb_enq_alt_def
+  apply(wp_once)+
+  apply(subst notfull)+
+  apply(wp_once)+
+  apply(auto simp:fun_upd_def)
+       prefer 6 using c_rb_valid_def apply blast
+      prefer 5 using c_rb_valid_def less_imp_le word_le_def apply blast
+     prefer 4 using c_rb_valid_def unat_gt_0 apply fastforce 
+    prefer 3 apply (simp add: int_unat)
+   prefer 2 apply (simp add: int_unat)
+  using CleanQ_SimpleQ.c_ring_ptr_different by blast
+
+
+lemma c_rb_enq_state_update_ring2:
+  "\<lbrace> \<lambda>s. c_rb_valid s rb \<and> s0 = s  \<and> rb0 = rb_C_to_CleanQ_RB s rb   \<rbrace>
+   rb_enq_c_fun rb b
+   \<lbrace> \<lambda> r s.  (r = ERR_OK \<or> r = ERR_QUEUE_FULL) \<and> 
+         (if r = ERR_OK then (\<forall>i < size rb0. ring (rb_C_to_CleanQ_RB s rb) i = ring (rb_enq b rb0) i) 
+         else s = s0) \<rbrace>!"
+  unfolding rb_enq_c_fun_def  rb_C_to_CleanQ_RB_def rb_enq_equiv rb_enq_alt_def
+  apply(wp_once)+
+  apply(simp add:rb_can_enq_c_fun_def)
+  apply(wp_once)+
+  apply(auto simp:fun_upd_def)
+  using CleanQ_SimpleQ.c_ring_ptr_different apply blast
+  unfolding c_rb_valid_def
+  apply (simp_all add: int_unat)
+  using unat_gt_0 apply fastforce
+  using less_imp_le word_le_def apply blast
+  using INT_MIN_MAX_lemmas(12) Suc_leI  unat_32word_leq_lt_lt apply blast
+  using unat_gt_0 by fastforce     
+  
+   
+
+lemma c_rb_enq_state_update:
+assumes notfull: " rb_can_enq_c_fun rb = return (1) "
+  shows "\<lbrace> \<lambda>s. c_rb_valid s rb \<and> s0 = s \<and> rb0 = rb_C_to_CleanQ_RB s rb  \<rbrace>
+           rb_enq_c_fun rb b
+         \<lbrace> \<lambda> r s. rb_C_to_CleanQ_RB s rb = rb_enq b rb0 \<rbrace>!"
+  (* doesn't work yet *)
+  oops
+
+
+(* ========================== *)
+(* BAD LEMMAS FOLLOW WHICH USE SORRY *)
+(*
+
+
+
+lemma ddd:
+  "unat (of_int (uint (head_C (heap_rb_C s0 rb)))) \<le> UINT_MAX"
+proof -
+  have X0: "unat (h::uint_t) \<le> UINT_MAX"
+    by(auto)
+  from X0 have X1:
+    "uint (h::uint_t) \<le> UINT_MAX"
+    by (metis (full_types) INT_MIN_MAX_lemmas(12) int_unat of_nat_le_iff)
+  from X1 have X2:
+    "unat (of_int (uint (h::uint_t))) \<le> UINT_MAX"
+    by (metis INT_MIN_MAX_lemmas(12) int_unat le_cases le_unat_uoi of_int_of_nat_eq)
+  show ?thesis 
+    by (metis INT_MIN_MAX_lemmas(12) dual_order.trans int_unat of_int_of_nat_eq order_refl unat_le_helper)
+qed
+
+lemma hack:
+  assumes xbound: "x < unat (size_C (heap_rb_C s0 rb))" 
+    and valid: "c_rb_valid s0 rb"
+  shows
+  "ring_C (heap_rb_C s0 rb) +\<^sub>p int x = ring_C (heap_rb_C s0 rb) +\<^sub>p uint (head_C (heap_rb_C s0 rb)) \<longleftrightarrow>  x = unat (head_C (heap_rb_C s0 rb))"
+  unfolding ptr_add_def
+proof (auto)
+  assume p: "of_nat x * (0x40::64 word) = of_int (uint (head_C (heap_rb_C s0 rb))) * (0x40::64 word)"
+  show "x = unat (head_C (heap_rb_C s0 rb))"
+  proof -
+
+
+
+    from xbound have xlimnat:
+      "x \<le> 0xffffffff"
+      by (metis INT_MIN_MAX_lemmas(12) UINT_MAX_def dual_order.trans not_le order.asym)
+
+    from xbound have ofnatxless:
+      "of_nat x < size_C (heap_rb_C s0 rb)"
+      by (simp add: word_of_nat_less)
+     
+    from ofnatxless have xlim32:
+      "((of_nat x)::uint_t) \<le> 0xffffffff"
+      by (metis UINT_MAX_def of_nat_numeral word_and_le1 word_and_max_simps(3))
+
+    from xlim32 ofnatxless have 
+        "unat ((of_nat x)::ulong_t) = x"
+
+
+    have headlim32:
+      "(head_C (heap_rb_C s0 rb)) \<le> 0xffffffff"
+      by (metis word_and_le1 word_and_max_simps(3))
+
+    have unatheadlim32:
+      "unat (head_C (heap_rb_C s0 rb)) \<le> 0xffffffff"
+      using  UINT_MAX_def by auto
+
+    from xlimnat xlim32  have
+      "unat (of_nat x * (0x40::64 word)) = unat(of_nat x) * unat (0x40::64 word)"
+      sorry
+
+    from p have X0:
+      "((of_nat x)::64 word) = of_int (uint (head_C (heap_rb_C s0 rb)))"
+      sorry
+    from X0 have X1:
+      "unat ((of_nat x)::64 word) = unat (of_int (uint (head_C (heap_rb_C s0 rb))))"
+      sorry
+
+    show ?thesis
+      sorry
+  qed
+next
+  assume p: "x = unat (head_C (heap_rb_C s0 rb))"
+  show "of_nat (unat (head_C (heap_rb_C s0 rb))) * (0x40::64 word) = of_int (uint (head_C (heap_rb_C s0 rb))) * (0x40::64 word)"
+    by (metis int_unat of_int_of_nat_eq)
+qed
+
+
+(* !!!  THIS ONE IS BAD !!! *)
+
+
+lemma hack:
+  "ring_C (heap_rb_C s0 rb) +\<^sub>p int x = ring_C (heap_rb_C s0 rb) +\<^sub>p uint (head_C (heap_rb_C s0 rb)) \<longleftrightarrow>  x = unat (head_C (heap_rb_C s0 rb))"
+  unfolding ptr_add_def
+proof (auto)
+  assume p: "of_nat x * (0x40::64 word) = of_int (uint (head_C (heap_rb_C s0 rb))) * (0x40::64 word)"
+  show "x = unat (head_C (heap_rb_C s0 rb))"
+  proof -
+
+    from p have X0:
+      "((of_nat x)::64 word) = of_int (uint (head_C (heap_rb_C s0 rb)))"
+      sorry
+    from X0 have X1:
+      "unat ((of_nat x)::64 word) = unat (of_int (uint (head_C (heap_rb_C s0 rb))))"
+      sorry
+
+    show ?thesis
+      sorry
+  qed
+next
+  assume p: "x = unat (head_C (heap_rb_C s0 rb))"
+  show "of_nat (unat (head_C (heap_rb_C s0 rb))) * (0x40::64 word) = of_int (uint (head_C (heap_rb_C s0 rb))) * (0x40::64 word)"
+    by (metis int_unat of_int_of_nat_eq)
+qed
+
+lemma c_rb_enq_correct:
+  "\<lbrace> \<lambda>s. c_rb_valid s rb \<and> s0 = s \<and> rb0 = rb_C_to_CleanQ_RB s rb  \<rbrace>
+      rb_enq_c_fun rb b
+   \<lbrace> \<lambda> r s. (r = ERR_OK \<or> r = ERR_QUEUE_FULL) \<and> 
+              (if r = ERR_OK then rb_C_to_CleanQ_RB s rb = rb_enq b rb0 else s = s0) \<rbrace>!"
+  unfolding rb_enq_c_fun_def  rb_C_to_CleanQ_RB_def rb_enq_equiv rb_enq_alt_def
+  apply(wp_once)+
+  apply(simp add:rb_can_enq_c_fun_def)
+  apply(wp_once)+
+  apply(auto simp:fun_upd_def c_rb_valid_def  unat_32word_succ_mod word_less_nat_alt Suc_le_eq unat_32word_leq_lt_lt)
+  apply(subst hack)
+  using word_le_def word_le_less_eq word_less_nat_alt by blast+
+
+
+
+*)
 (* ####################################################### *)
 
 
